feat: start to prove from_list

src/MVector.thy
@@ -68,10 +68,86 @@ lemma execute_read: "execute (read v i) h = (get_at h v i, h)"
 lemma execute_writ: "execute (writ r i v) h = ((), set_at r i v h)"
   by (simp add: writ_def)
 
+(*
+fast implementation
+
 definition from_list :: "'a::heap list \<Rightarrow> 'a mvector io" where
   "from_list xs = fold (\<lambda>(i,x) m. m \<bind> (\<lambda>vec. writ vec i x \<bind> (\<lambda>_. return vec))) (enumerate 0 xs) (new (size xs))"
+*)
+
+primrec from_list_pr :: "'a::heap mvector \<Rightarrow> 'a::heap list \<Rightarrow> nat \<Rightarrow> 'a mvector io" where
+  "from_list_pr mvec [] n = return mvec"
+| "from_list_pr mvec (x#xs) n = writ mvec n x \<bind> (\<lambda>_. from_list_pr mvec xs (Suc n))"
+
+definition from_list :: "'a::heap list \<Rightarrow> 'a mvector io" where
+  "from_list xs = new (size xs) \<bind> (\<lambda>mvec. from_list_pr mvec xs 0)"
 
 definition to_list :: "'a::heap mvector \<Rightarrow> 'a list io" where
   "to_list vec = (let s = size_of_mvector vec in mapM (\<lambda>i. read vec (nat i)) [0..int s])"
+
+definition set_over :: "'a::heap mvector \<Rightarrow> 'a::heap list \<Rightarrow> heap \<Rightarrow> heap" where
+  "set_over r xs h = h \<lparr> memory := (\<lambda>i. if lim h < i \<and> i < lim h + Addr (size xs) then to_nat (get_at h r (nat_of_addr (i - lim h))) else memory h i) \<rparr>"
+
+primrec snoc :: "'a list \<Rightarrow> 'a \<Rightarrow> 'a list" where
+  "snoc [] x = [x]"
+| "snoc (y#ys) x = y # snoc ys x"
+
+lemma snoc_length: "length (snoc ys y) = Suc (length ys)"
+  by (induct ys, auto)
+
+lemma snoc_induct:
+  assumes "P []"
+  and "\<And>xs y. P xs \<Longrightarrow> P (snoc xs y)"
+  shows "P xs"
+  apply (induct "size xs" arbitrary: xs)
+  apply (simp add: assms(1))
+proof-
+  have cons_snoc: "\<And>(a :: 'a list) x xs. a = x # xs \<Longrightarrow> \<exists>y ys. a = snoc ys y"
+  proof-
+    fix a :: "'a list" and x xs
+    show cons_snoc: "a = x # xs \<Longrightarrow> \<exists>y ys. a = snoc ys y"
+      apply (induct a arbitrary: x xs, auto)
+    proof-
+      fix x :: 'a and xs
+      assume "\<And>x (xsa :: 'a list). xs = x # xsa \<Longrightarrow> \<exists>y ys. x # xsa = snoc ys y"
+      show "\<exists>y ys. x # xs = snoc ys y"
+        apply (cases xs)
+        apply (metis snoc.simps(1))
+        by (metis \<open>\<And>xsa xa. xs = xa # xsa \<Longrightarrow> \<exists>y ys. xa # xsa = snoc ys y\<close> snoc.simps(2))
+    qed
+  qed
+
+  fix x and xs :: "'a list"
+  assume "\<And>xs. x = length xs \<Longrightarrow> P xs"
+  and "Suc x = length xs"
+  obtain y ys where "xs = y # ys"
+    by (meson Suc_length_conv \<open>Suc x = length xs\<close>)
+  then obtain z zs where "xs = snoc zs z"
+    using cons_snoc by blast
+  hence "x = length zs"
+    by (simp add: Suc_inject \<open>Suc x = length xs\<close> snoc_length)
+  show "P xs"
+    by (simp add: \<open>\<And>xs. x = length xs \<Longrightarrow> P xs\<close> \<open>x = length zs\<close> \<open>xs = snoc zs z\<close> assms(2))
+qed
+
+lemma from_list_snoc: "execute (from_list (snoc ys y)) h = execute (do {
+  mvec \<leftarrow> new (Suc (size ys));
+  _ \<leftarrow> from_list_pr mvec ys 0;
+  writ mvec (Suc (size ys)) y;
+  return mvec
+}) h"
+  apply (simp add: from_list_def snoc_length)
+  sorry
+
+lemma execute_from_list: "execute (from_list xs) h = (case alloc (size xs) h of (mvec,h0) \<Rightarrow> (mvec, fold (\<lambda>(i,x) h. set_at mvec i x h) (enumerate 0 xs) h0))"
+  apply (induct xs arbitrary: h rule: snoc_induct)
+  apply (simp add: from_list_def new_def)
+proof-
+  fix xs :: "'a list" and y h
+  assume "\<And>h. execute (from_list xs) h = (case alloc (length xs) h of (mvec, h0) \<Rightarrow> (mvec, fold (\<lambda>(x, y). set_at mvec x y) (enumerate 0 xs) h0))"
+
+  show "execute (from_list (snoc xs y)) h = (case alloc (length (snoc xs y)) h of (mvec, h0) \<Rightarrow> (mvec, fold (\<lambda>(x, y). set_at mvec x y) (enumerate 0 (snoc xs y)) h0))"
+    sorry
+qed
 
 end
